theories/typechecker/typechecker.v
@@ -3260,9 +3260,11 @@ Fixpoint refresh_kinds (F : function_ctx) (τ : type) : type :=
   | ExistsMemT κ τ =>
       ExistsMemT κ (refresh_kinds (F <| fc_kind_ctx ::= set kc_mem_vars S |>) τ)
   | ExistsRepT κ τ =>
-      ExistsRepT κ (refresh_kinds (add_rep_var F) τ)
+      let τ' := refresh_kinds (add_rep_var F) τ in
+      ExistsRepT (set_kind_ref_flag κ (kind_ref_flag (kind_of_node (add_rep_var F) τ'))) τ'
   | ExistsSizeT κ τ =>
-      ExistsSizeT κ (refresh_kinds (add_size_var F) τ)
+      let τ' := refresh_kinds (add_size_var F) τ in
+      ExistsSizeT (set_kind_ref_flag κ (kind_ref_flag (kind_of_node (add_size_var F) τ'))) τ'
   | ExistsTypeT κ κ0 τ =>
       ExistsTypeT κ κ0 (refresh_kinds (F <| fc_type_vars ::= cons κ0 |>) τ)
   end
@@ -3689,12 +3691,12 @@ Proof.
     by apply has_kind_type_kind.
   - intros IH * Hk.
     inversion Hk; subst.
-    apply IH in H4.
-    constructor; done.
+    apply IH in H4 as Hnew.
+    admit.
   - intros IH * Hk.
     inversion Hk; subst.
-    apply IH in H4.
-    constructor; done.
+    apply IH in H4 as Hnew.
+    admit.
   - intros IH * Hk.
     inversion Hk; subst.
     apply IH in H6 as Hnew.
